STLCWA progress completed.

STLCWA.v
@@ -1,4 +1,5 @@
-Require Import Maps.
+
+Require Import SfLib.
 
 
 Module STLCARITH.
@@ -7,6 +8,7 @@ Inductive ty : Type :=
     | TArrow : ty -> ty -> ty
     | TNat : ty.
 
+    Hint Constructors ty.
 Inductive tm : Type :=
     | tvar : id -> tm 
     | tapp : tm -> tm -> tm
@@ -19,54 +21,317 @@ Inductive tm : Type :=
 
 (* Weak Typing. 0 as False, others are true. *)
 
-Inductive TyContext : Type :=
-    | empty : TyContext 
-    | update : id -> ty -> TyContext -> TyContext.
+    Hint Constructors tm.
+
+Inductive Context {type : Type} : Type :=
+    | empty : Context
+    | update : id -> type -> Context -> Context.
     
-Fixpoint byContext (ctx : TyContext) (i : id) : option ty :=
+    Hint Constructors Context.
+Fixpoint byContext (ctx : Context) (i : id) : option ty :=
     match ctx with 
         | empty => None
         | update x Ty ctx' =>
             if (eq_id_dec i x) then Some Ty else byContext ctx' i
             end.
 
-Reserved Notation "Gamma '|-' t '\in' T" (at level 40).            
+Reserved Notation "Gamma '|=' t '\in' T" (at level 40).            
 
-Inductive has_type : TyContext -> tm -> ty -> Type :=
+Inductive has_type : Context -> tm -> ty -> Type :=
     | tyVar : 
         forall G i T,
             byContext G i = Some T ->
-            G |- tvar i \in T
+            G |= tvar i \in T
     | tyApp :
         forall Gamma a b G T,
-        Gamma |- a \in TArrow G T ->
-        Gamma |- b \in G ->
-        Gamma |- tapp a b \in T
+        Gamma |= a \in TArrow G T ->
+        Gamma |= b \in G ->
+        Gamma |= tapp a b \in T
     | tyAbs :
         forall Gamma i x G T,
-        update i G Gamma |- x \in T ->
-        Gamma |- tabs i T x \in TArrow G T
+        update i G Gamma |= x \in T ->
+        Gamma |= tabs i G x \in TArrow G T
     | tyNat :
         forall i Gamma,
-        Gamma |- tnat i \in TNat
+        Gamma |= tnat i \in TNat
     | tySucc :
         forall x Gamma,
-        Gamma |- x \in TNat ->
-        Gamma |- tsucc x \in TNat
+        Gamma |= x \in TNat ->
+        Gamma |= tsucc x \in TNat
     | tyPred :
         forall x Gamma,
-        Gamma |- x \in TNat ->
-        Gamma |- tpred x \in TNat
+        Gamma |= x \in TNat ->
+        Gamma |= tpred x \in TNat
     | tyMult :
         forall x y Gamma,
-        Gamma |- x \in TNat ->
-        Gamma |- y \in TNat ->
-        Gamma |- tmult x y \in TNat
+        Gamma |= x \in TNat ->
+        Gamma |= y \in TNat ->
+        Gamma |= tmult x y \in TNat
     | tyIf :
         forall t t0 t1 Gamma T,
-        Gamma |- t0 \in T ->
-        Gamma |- t1 \in T ->
-        Gamma |- t \in TNat ->
-        Gamma |- tif0 t t0 t1 \in T
-    where "Gamma '|-' t '\in' T " := (has_type Gamma t T).
+        Gamma |= t0 \in T ->
+        Gamma |= t1 \in T ->
+        Gamma |= t \in TNat ->
+        Gamma |= tif0 t t0 t1 \in T
+    where "Gamma '|=' t '\in' T " := (has_type Gamma t T).
+
+    Hint Constructors has_type.
+    Reserved Notation "'[' x ':=' s ']' t" (at level 20).
+    
+    
+
+Fixpoint subst (i : id) (t org : tm) : tm :=
+    match org with
+        | tvar j => if(eq_id_dec i j) then t else org
+        | tapp a b => tapp ([i := t] a) ([i := t] b)
+        | tabs x T y => tabs x T (if (eq_id_dec i x) then y else ([i := t] y))
+        | tsucc x => tsucc ([i := t] x)
+        | tpred y => tpred ([i := t] y)
+        | tmult x y => tmult ([i := t] x) ([i := t] y)
+        | tif0 x t0 t1 => tif0 ([i := t] x) ([i := t] t0) ([i := t] t1)
+        | _ => org
+        end
+        where "'[' x ':=' s ']' t" := (subst x s t).
+
+
+Inductive value : tm -> Prop :=
+    | vnat : 
+        forall n,
+            value (tnat n)
+    | vabs :
+        forall x T y,
+            value (tabs x T y).
+
+Reserved Notation "t '==>' t'" (at level 40).
+        
+    Hint Constructors value.
+Inductive step : tm -> tm -> Prop :=
+    | ST_AppAbs :
+        forall abs abs' arg,
+        abs ==> abs' ->
+        tapp abs arg ==> tapp abs' arg
+    | ST_AppArg :
+        forall abs arg arg',
+        value abs ->
+        arg ==> arg' ->
+        tapp abs arg ==> tapp abs arg'
+    | ST_App :
+        forall x T y arg,
+        value arg ->
+        tapp (tabs x T y) arg ==> [x := arg] y
+    | ST_Succ0 :
+        forall n n',
+        n ==> n' ->
+        tsucc n ==> tsucc n'
+    | ST_Succ1 :
+        forall n,
+        tsucc (tnat n) ==> tnat (S n)
+    | ST_Pred0 :
+        forall n n',
+        n ==> n' ->
+        tpred n ==> tpred n'
+    | ST_Pred1 :
+        forall n,
+        tpred (tnat n) ==> tnat (pred n)
+    | ST_Mult0 :
+        forall n0 n0' n1,
+        n0 ==> n0' ->
+        tmult n0 n1 ==> tmult n0' n1
+    | ST_Mult1 :
+        forall n0 n1 n1',
+        value n0 ->
+        n1 ==> n1' ->
+        tmult n0 n1 ==> tmult n0 n1'
+    | ST_Mult2 :
+        forall n0 n1,
+        tmult (tnat n0) (tnat n1) ==> tnat (n0 * n1)
+    | ST_If0 :
+        forall t t' t0 t1,
+        t ==> t' ->
+        tif0 t t0 t1 ==> tif0 t' t0 t1
+    | ST_IfFalse :
+        forall t0 t1,
+        tif0 (tnat 0) t0 t1 ==> t1
+    | ST_IfTrue :
+        forall t t0 t1,
+        t <> 0 ->
+        tif0 (tnat t) t0 t1 ==> t0
+    where "t '==>' t'" := (step t t').
+
+    Hint Constructors step.
+
+    Theorem deterministic_step :
+        deterministic step.
+    
+    unfold deterministic.
+    intros x y1 y2 h.
+    generalize dependent y2.
+    elim h; intros.
+
+    inversion H1; subst. pose (H0 _ H5). rewrite e; auto.
+    inversion H4; subst. inversion H.
+
+    Abort.
+
+    Lemma value_cant_step:
+        forall n n',
+        value n ->
+        n ==> n' ->
+        False.
+    intros n n' h.
+    generalize dependent n'.
+    elim h; subst; intros.
+    inversion H. inversion H.
+Qed.
+
+
+
+Ltac value_no_stepping_ :=
+    match goal with
+     | [ H1 : tabs ?X ?T ?Y ==> ?Z |- _ ] => inversion H1
+     | [ H1 : tnat ?N ==> ?Z |- _ ] => inversion H1
+     | [ H1 : value ?X, H2 : ?X ==> ?Z |- _ ] => destruct (value_cant_step _ _ H1 H2)
+     end.
+
+Ltac value_no_stepping := repeat value_no_stepping_.
+
+Theorem deterministic_step :
+     deterministic step.
+     
+     unfold deterministic.
+     intros x y1 y2 h.
+     generalize dependent y2.
+     elim h; intros until y2; intro HH;
+     inversion HH; subst; try value_no_stepping; auto.
+
+     pose (H0 _ H4). rewrite e; auto.
+
+     pose (H1 _ H6). rewrite e; auto.
+
+     rewrite (H0 _ H2); auto.
+
+     rewrite (H0 _ H2); auto.
+
+     rewrite (H0 _ H4); auto.
+
+     rewrite (H1 _ H6); auto.
+
+     rewrite (H0 _ H5); auto.
+
+     destruct (H3 eq_refl).
+     destruct (H eq_refl).
+
+Qed.
+
+Lemma canonical_forms_bool :
+    forall t,
+    empty |= t \in TNat ->
+    value t ->
+    (exists i, t = tnat i).
+
+    intros. inversion H0; subst. 
+    exists n; auto.
+    inversion H; subst.
+Qed.
+
+Lemma canonical_forms_fun :
+    forall t G T,
+        empty |= t \in TArrow G T ->
+        value t ->
+        (exists x v, t = tabs x G v).
+
+    intros. inversion H0; subst.
+    inversion H.
+    exists x. exists y. inversion H; subst. auto.
+
+Qed.
+
+Hint Unfold byContext.
+
+Theorem progress :
+    forall t T,
+        empty |= t \in T ->
+        value t \/ (exists t', t ==> t').
+
+    intro. elim t; intros.
+    inversion H; subst.  inversion H2.
+
+    inversion H1; subst. 
+    right.
+    destruct (H _ H5). 
+    destruct (H0 _ H7). 
+    inversion H2; subst. inversion H5.
+    exists ([x := t1] y). eauto.
+
+    destruct H3. exists (tapp t0 x). eauto.
+    destruct H2. exists (tapp x t1). eauto.
+    
+    left; eauto.
+    left; eauto.
+
+    right. inversion H0; subst. 
+    destruct (H _ H3). 
+    inversion H1; subst.
+    exists (tnat (S n)). eauto.
+    inversion H3.
+    destruct H1.
+    exists (tsucc x). eauto.
+
+    right. inversion H0; subst.
+    destruct (H _ H3). inversion H1; subst.
+    exists (tnat (pred n)); eauto.
+    inversion H3.
+
+    destruct H1.
+    exists (tpred x). eauto.
+
+    right. inversion H1; subst.
+    destruct  (H _ H5). destruct (H0 _ H7).
+    inversion H2; inversion H3; subst.
+    exists (tnat (n * n0)); eauto.
+
+    inversion H7. inversion H5. inversion H5.
+
+    destruct H3.
+    exists (tmult t0 x). eauto.
+
+    destruct H2.
+    exists (tmult x t1). eauto.
+
+    right. inversion H2; subst. 
+    destruct (H _ H10). inversion H3; subst.
+    destruct n. exists t2; eauto.
+    assert (S n <> 0); eauto.
+    inversion H10. 
+    destruct H3.
+    exists (tif0 x t1 t2); eauto.
+Qed.
+
+
+
+
+
+
+
+    
+
+
+
+     
+     
+
+
+
+
+
+
+
+
+
+
+
+
+
+
+
         
